Cpc/Proofs/Rules/Str_indexof_prefix_concat.lean
@@ -1,0 +1,23 @@
+module
+
+public import Cpc.Proofs.RuleSupport.Support
+import all Cpc.Proofs.RuleSupport.Support
+
+open Eo
+open SmtEval
+open Smtm
+
+set_option linter.unusedVariables false
+set_option maxHeartbeats 10000000
+
+
+public theorem cmd_step_str_indexof_prefix_concat_properties
+    (M : SmtModel) (hM : model_wf M)
+    (s : CState) (args : CArgList) (premises : CIndexList) :
+  cmdTranslationOk (CCmd.step CRule.str_indexof_prefix_concat args premises) ->
+  AllHaveBoolType (premiseTermList s premises) ->
+  __eo_typeof (__eo_cmd_step_proven s CRule.str_indexof_prefix_concat args premises) = Term.Bool ->
+  StepRuleProperties M (premiseTermList s premises)
+    (__eo_cmd_step_proven s CRule.str_indexof_prefix_concat args premises) :=
+by
+  sorry
